lagrange out of domain mid => high

src/Field.ec
@@ -1,6 +1,7 @@
 pragma Goals:printall.
 
 require import AllCore.
+require import Constants.
 require import Int.
 require import IntDiv.
 require import StdOrder.
@@ -17,20 +18,23 @@ clone include ZModField
   rename "zmod" as "F"
   rename "ZModp" as "Zq".
 end FieldQ.
+
+axiom q_eq_fieldq_p: Q = FieldQ.p.
+axiom r_eq_fieldr_p: R = FieldR.p.    
+lemma prime_q : prime Q by rewrite q_eq_fieldq_p; exact FieldQ.prime_p.
+lemma prime_r : prime R by rewrite r_eq_fieldr_p; exact FieldR.prime_p.
   
 op (^) (x : FieldR.F) (k : int) = FieldR.exp x k axiomatized by RexpE.
 
-(* op OMEGAFr = inFr OMEGA axiomatized by omegaFrE. *)
-(* op DOMAIN_SIZEFr = inFr DOMAIN_SIZE axiomatized by domain_sizeFrE. *)
+op OMEGAFr = FieldR.inF Constants.OMEGA axiomatized by omegaFrE.
+op DOMAIN_SIZEFr = FieldR.inF DOMAIN_SIZE axiomatized by domain_sizeFrE.
 
-(* lemma omega_eq_omegaFr : asint OMEGAFr = OMEGA. *)
-(* proof. *)
-(*   rewrite omegaFrE /asint /inFr; have ->: OMEGA %% R = OMEGA by smt. *)
-(*   rewrite Sub.insubdK //; smt. *)
-(* qed. *)
+lemma omega_eq_omegaFr : FieldR.asint OMEGAFr = OMEGA. 
+proof.
+  rewrite omegaFrE FieldR.inFK /OMEGA -r_eq_fieldr_p /Constants.R. progress. 
+qed.
 
-(* lemma domain_eq_domainFr : asint DOMAIN_SIZEFr = DOMAIN_SIZE. *)
-(* proof. *)
-(*   rewrite domain_sizeFrE /asint /inFr; have ->: DOMAIN_SIZE %% R = DOMAIN_SIZE by smt. *)
-(*   rewrite Sub.insubdK //; smt. *)
-(* qed. *)
+lemma domain_eq_domainFr : FieldR.asint DOMAIN_SIZEFr = DOMAIN_SIZE.
+proof.
+  rewrite domain_sizeFrE FieldR.inFK /DOMAIN_SIZE -r_eq_fieldr_p /Constants.R. progress.
+qed.
